{"nbformat":4,"nbformat_minor":0,"metadata":{"colab":{"provenance":[],"authorship_tag":"ABX9TyPejrrxhcfD5R8iBBn+2KeU"},"kernelspec":{"name":"python3","display_name":"Python 3"},"language_info":{"name":"python"}},"cells":[{"cell_type":"markdown","source":["1) find gradient of  \tÎ¦=(x^2)yz"],"metadata":{"id":"yUhzQ4WnIBvU"}},{"cell_type":"code","source":["from sympy.physics.vector import *\n","from sympy import var\n","var('x,y,z')\n","v= ReferenceFrame ('v')\n","F=v[0]**2*v[1]*v[2]\n","G=gradient(F,v)\n","F=F.subs([(v[0],x),(v[1],y),(v[2],z)])\n","print(\"given scalar function F=\")\n","display(F)\n","G=G.subs([(v[0],x),(v[1],y),(v[2],z)])\n","print(\"Gradient of F=\")\n","display(G)"],"metadata":{"colab":{"base_uri":"https://localhost:8080/","height":94},"id":"FsMsQbH0Il8s","executionInfo":{"status":"ok","timestamp":1713863207920,"user_tz":-330,"elapsed":500,"user":{"displayName":"Junaid Umar","userId":"00471791025673001364"}},"outputId":"6c8856f0-404f-4f04-edda-57fd9ea84997"},"execution_count":null,"outputs":[{"output_type":"stream","name":"stdout","text":["given scalar function F=\n"]},{"output_type":"display_data","data":{"text/plain":["x**2*y*z"],"text/latex":"$\\displaystyle x^{2} y z$"},"metadata":{}},{"output_type":"stream","name":"stdout","text":["Gradient of F=\n"]},{"output_type":"display_data","data":{"text/plain":["2*x*y*z*v.x + x**2*z*v.y + x**2*y*v.z"],"text/latex":"$\\displaystyle 2 x y z\\mathbf{\\hat{v}_x} + x^{2} z\\mathbf{\\hat{v}_y} + x^{2} y\\mathbf{\\hat{v}_z}$"},"metadata":{}}]},{"cell_type":"markdown","source":["2) find Divergence of F=[x^2y]i + [yz^2]j + [x^2z]k"],"metadata":{"id":"1BDnX43ENZbp"}},{"cell_type":"code","source":["from sympy.physics.vector import *\n","from sympy import var\n","var('x,y,z')\n","v= ReferenceFrame ('v')\n","F=v[0]**2*v[1]*v.x+v[1]*v[2]**2*v.y+v[0]**2*v[2]*v.z\n","G=divergence (F,v)\n","F=F.subs([(v[0],x),(v[1],y),(v[2],z)])\n","print(\"given scalar function F=\")\n","display(F)\n","G=G.subs([(v[0],x),(v[1],y),(v[2],z)])\n","print(\"Divergence of F=\")\n","display(G)"],"metadata":{"colab":{"base_uri":"https://localhost:8080/","height":94},"id":"22IaK4UXOD_L","executionInfo":{"status":"ok","timestamp":1713863941346,"user_tz":-330,"elapsed":504,"user":{"displayName":"Junaid Umar","userId":"00471791025673001364"}},"outputId":"b9fb4855-cdb3-4db5-c1ee-540b04dad853"},"execution_count":null,"outputs":[{"output_type":"stream","name":"stdout","text":["given scalar function F=\n"]},{"output_type":"display_data","data":{"text/plain":["x**2*y*v.x + y*z**2*v.y + x**2*z*v.z"],"text/latex":"$\\displaystyle x^{2} y\\mathbf{\\hat{v}_x} + y z^{2}\\mathbf{\\hat{v}_y} + x^{2} z\\mathbf{\\hat{v}_z}$"},"metadata":{}},{"output_type":"stream","name":"stdout","text":["Divergence of F=\n"]},{"output_type":"display_data","data":{"text/plain":["x**2 + 2*x*y + z**2"],"text/latex":"$\\displaystyle x^{2} + 2 x y + z^{2}$"},"metadata":{}}]},{"cell_type":"markdown","source":["3) prove that the vector (yz-x^2)i + (4y-(z^2)x)j + (2xz-4z)k is solenoidal"],"metadata":{"id":"emkNdTW-QHDA"}},{"cell_type":"code","source":["from sympy.physics.vector import *\n","from sympy import var\n","var('x,y,z')\n","v= ReferenceFrame ('v')\n","F=((v[1]*v[2]-v[0]**2))*v.x + (4*v[1]-(v[2]**2)*v[0])*v.y + (2*v[0]*v[2]-4*v[2])*v.z\n","G=divergence (F,v)\n","F=F.subs([(v[0],x),(v[1],y),(v[2],z)])\n","print(\"given scalar function F=\")\n","display(F)\n","G=G.subs([(v[0],x),(v[1],y),(v[2],z)])\n","print(\"Divergence of F=\")\n","display(G)"],"metadata":{"colab":{"base_uri":"https://localhost:8080/","height":93},"id":"1Rgc9GVzQHPW","executionInfo":{"status":"ok","timestamp":1713865078240,"user_tz":-330,"elapsed":662,"user":{"displayName":"Junaid Umar","userId":"00471791025673001364"}},"outputId":"fc838e0c-31c3-45ff-b24c-8fb09bf4b7ab"},"execution_count":null,"outputs":[{"output_type":"stream","name":"stdout","text":["given scalar function F=\n"]},{"output_type":"display_data","data":{"text/plain":["(-x**2 + y*z)*v.x + (-x*z**2 + 4*y)*v.y + (2*x*z - 4*z)*v.z"],"text/latex":"$\\displaystyle (- x^{2} + y z)\\mathbf{\\hat{v}_x} + (- x z^{2} + 4 y)\\mathbf{\\hat{v}_y} + (2 x z - 4 z)\\mathbf{\\hat{v}_z}$"},"metadata":{}},{"output_type":"stream","name":"stdout","text":["Divergence of F=\n"]},{"output_type":"display_data","data":{"text/plain":["0"],"text/latex":"$\\displaystyle 0$"},"metadata":{}}]},{"cell_type":"markdown","source":["4)Find the curl of F=[xy^2]i + [2(x^2)yz]j - [3yz^2]k"],"metadata":{"id":"rhXefqkvSqnv"}},{"cell_type":"code","source":["from sympy.physics.vector import *\n","from sympy import var\n","var('x,y,z')\n","v= ReferenceFrame ('v')\n","F=(v[0]*v[1]**2)*v.x + 2*((v[0]**2)*v[1]*v[2])*v.y - (3*v[1]*v[2]**2)*v.z\n","G=curl (F,v)\n","F=F.subs([(v[0],x),(v[1],y),(v[2],z)])\n","print(\"given vector function F=\")\n","display(F)\n","G=G.subs([(v[0],x),(v[1],y),(v[2],z)])\n","print(\"Curl of F=\")\n","display(G)"],"metadata":{"colab":{"base_uri":"https://localhost:8080/","height":94},"id":"08cqyJi_SqxX","executionInfo":{"status":"ok","timestamp":1713865601978,"user_tz":-330,"elapsed":541,"user":{"displayName":"Junaid Umar","userId":"00471791025673001364"}},"outputId":"d4a47eeb-6796-4cf0-e763-656c17d37e76"},"execution_count":null,"outputs":[{"output_type":"stream","name":"stdout","text":["given vector function F=\n"]},{"output_type":"display_data","data":{"text/plain":["x*y**2*v.x + 2*x**2*y*z*v.y - 3*y*z**2*v.z"],"text/latex":"$\\displaystyle x y^{2}\\mathbf{\\hat{v}_x} + 2 x^{2} y z\\mathbf{\\hat{v}_y} -  3 y z^{2}\\mathbf{\\hat{v}_z}$"},"metadata":{}},{"output_type":"stream","name":"stdout","text":["Curl of F=\n"]},{"output_type":"display_data","data":{"text/plain":["(-2*x**2*y - 3*z**2)*v.x + (4*x*y*z - 2*x*y)*v.z"],"text/latex":"$\\displaystyle (- 2 x^{2} y - 3 z^{2})\\mathbf{\\hat{v}_x} + (4 x y z - 2 x y)\\mathbf{\\hat{v}_z}$"},"metadata":{}}]},{"cell_type":"markdown","source":["5) show that F=(4xy-z^3)i + 2x^2j + 3xz^2k  is irrotational"],"metadata":{"id":"huAyBV0jUhU5"}},{"cell_type":"code","source":["from sympy.physics.vector import *\n","from sympy import var\n","var('x,y,z')\n","v= ReferenceFrame ('v')\n","F=(4*v[0]*v[1]-v[2]**3)*v.x + 2*(v[0]**2)*v.y - (3*v[0]*v[2]**2)*v.z\n","G=curl (F,v)\n","F=F.subs([(v[0],x),(v[1],y),(v[2],z)])\n","print(\"given scalar function F=\")\n","display(F)\n","G=G.subs([(v[0],x),(v[1],y),(v[2],z)])\n","print(\"Curl of F=\")\n","display(G)"],"metadata":{"colab":{"base_uri":"https://localhost:8080/","height":93},"id":"k6hURalNUhcm","executionInfo":{"status":"ok","timestamp":1713865402044,"user_tz":-330,"elapsed":1153,"user":{"displayName":"Junaid Umar","userId":"00471791025673001364"}},"outputId":"4b21ec41-0f9a-472b-bc99-9ad921feb451"},"execution_count":null,"outputs":[{"output_type":"stream","name":"stdout","text":["given scalar function F=\n"]},{"output_type":"display_data","data":{"text/plain":["(4*x*y - z**3)*v.x + 2*x**2*v.y - 3*x*z**2*v.z"],"text/latex":"$\\displaystyle (4 x y - z^{3})\\mathbf{\\hat{v}_x} + 2 x^{2}\\mathbf{\\hat{v}_y} -  3 x z^{2}\\mathbf{\\hat{v}_z}$"},"metadata":{}},{"output_type":"stream","name":"stdout","text":["Curl of F=\n"]},{"output_type":"display_data","data":{"text/plain":["0"],"text/latex":"$\\displaystyle 0$"},"metadata":{}}]},{"cell_type":"markdown","source":["6) if u=x+y+z, v=x^2+y^2+z^2, w=yz+zx+xy, find grad u, grad v, grad z"],"metadata":{"id":"C2NBNT_uWn-Y"}},{"cell_type":"code","source":["from sympy.physics.vector import *\n","from sympy import var\n","var('x,y,z')\n","v= ReferenceFrame ('v')\n","u=v[0]+v[1]+v[2]\n","Gu=gradient(u,v)\n","u=u.subs([(v[0],x),(v[1],y),(v[2],z)])\n","print(\"given scalar function u=\")\n","display(u)\n","Gu=Gu.subs([(v[0],x),(v[1],y),(v[2],z)])\n","print(\"gradient of u=\")\n","display(Gu)\n","\n","V=v[0]**2+v[1]**2+v[2]**2\n","GV=gradient(V,v)\n","V=V.subs([(v[0],x),(v[1],y),(v[2],z)])\n","print(\"given scalar function V=\")\n","display(V)\n","GV=GV.subs([(v[0],x),(v[1],y),(v[2],z)])\n","print(\"gradient of V=\")\n","display(GV)\n","\n","w=v[1]*v[2]+v[2]*v[0]+v[0]*v[1]\n","Gw=gradient(w,v)\n","w=w.subs([(v[0],x),(v[1],y),(v[2],z)])\n","print(\"given scalar function w=\")\n","display(w)\n","Gw=Gw.subs([(v[0],x),(v[1],y),(v[2],z)])\n","print(\"gradient of w=\")\n","display(Gw)"],"metadata":{"colab":{"base_uri":"https://localhost:8080/","height":248},"id":"ed5ApRzoWoIu","executionInfo":{"status":"ok","timestamp":1713866636883,"user_tz":-330,"elapsed":512,"user":{"displayName":"Junaid Umar","userId":"00471791025673001364"}},"outputId":"9710f1b5-a3b3-48f0-af81-98063cf94a9e"},"execution_count":null,"outputs":[{"output_type":"stream","name":"stdout","text":["given scalar function u=\n"]},{"output_type":"display_data","data":{"text/plain":["x + y + z"],"text/latex":"$\\displaystyle x + y + z$"},"metadata":{}},{"output_type":"stream","name":"stdout","text":["gradient of u=\n"]},{"output_type":"display_data","data":{"text/plain":["v.x + v.y + v.z"],"text/latex":"$\\displaystyle \\mathbf{\\hat{v}_x} + \\mathbf{\\hat{v}_y} + \\mathbf{\\hat{v}_z}$"},"metadata":{}},{"output_type":"stream","name":"stdout","text":["given scalar function V=\n"]},{"output_type":"display_data","data":{"text/plain":["x**2 + y**2 + z**2"],"text/latex":"$\\displaystyle x^{2} + y^{2} + z^{2}$"},"metadata":{}},{"output_type":"stream","name":"stdout","text":["gradient of V=\n"]},{"output_type":"display_data","data":{"text/plain":["2*x*v.x + 2*y*v.y + 2*z*v.z"],"text/latex":"$\\displaystyle 2 x\\mathbf{\\hat{v}_x} + 2 y\\mathbf{\\hat{v}_y} + 2 z\\mathbf{\\hat{v}_z}$"},"metadata":{}},{"output_type":"stream","name":"stdout","text":["given scalar function w=\n"]},{"output_type":"display_data","data":{"text/plain":["x*y + x*z + y*z"],"text/latex":"$\\displaystyle x y + x z + y z$"},"metadata":{}},{"output_type":"stream","name":"stdout","text":["gradient of w=\n"]},{"output_type":"display_data","data":{"text/plain":["(y + z)*v.x + (x + z)*v.y + (x + y)*v.z"],"text/latex":"$\\displaystyle (y + z)\\mathbf{\\hat{v}_x} + (x + z)\\mathbf{\\hat{v}_y} + (x + y)\\mathbf{\\hat{v}_z}$"},"metadata":{}}]},{"cell_type":"markdown","source":["7) find divF and curlF at the point(1,2,3), given that F= [(x^2)yz]i + [x(y^2)z]j + [xy(z^2)]k"],"metadata":{"id":"A0YQ1-WwbbX-"}},{"cell_type":"code","source":["from sympy.physics.vector import *\n","from sympy import var\n","var('x,y,z')\n","v= ReferenceFrame ('v')\n","F=v[0]**2*v[1]*v[2]*v.x + v[0]*(v[1]**2)*v[2]*v.y + v[0]*v[1]*v[2]**2*v.z\n","G=divergence (F,v)\n","F=F.subs([(v[0],x),(v[1],y),(v[2],z)])\n","print(\"given scalar function F=\")\n","display(F)\n","G=G.subs([(v[0],x),(v[1],y),(v[2],z)])\n","print(\"Divergence of F=\")\n","display(G)\n","G=G.subs([(x,1),(y,2),(z,3)])\n","print(\"divergence of F at (1,2,3) is\")\n","\n","F=v[0]**2*v[1]*v[2]*v.x + v[0]*(v[1]**2)*v[2]*v.y + v[0]*v[1]*v[2]**2*v.z\n","G=curl(F,v)\n","F=F.subs([(v[0],x),(v[1],y),(v[2],z)])\n","print(\"curl of F=\")\n","display(F)\n","G=G.subs([(x,1),(y,2),(z,3)])\n","print(\"divergence of F at(1,2,3) is\")\n","display(G)"],"metadata":{"colab":{"base_uri":"https://localhost:8080/","height":189},"id":"TiSO8ZMrbbhu","executionInfo":{"status":"ok","timestamp":1713880975639,"user_tz":-330,"elapsed":1582,"user":{"displayName":"Junaid Umar","userId":"00471791025673001364"}},"outputId":"908f6a20-010d-4da4-8013-9128f40dc218"},"execution_count":null,"outputs":[{"output_type":"stream","name":"stdout","text":["given scalar function F=\n"]},{"output_type":"display_data","data":{"text/plain":["x**2*y*z*v.x + x*y**2*z*v.y + x*y*z**2*v.z"],"text/latex":"$\\displaystyle x^{2} y z\\mathbf{\\hat{v}_x} + x y^{2} z\\mathbf{\\hat{v}_y} + x y z^{2}\\mathbf{\\hat{v}_z}$"},"metadata":{}},{"output_type":"stream","name":"stdout","text":["Divergence of F=\n"]},{"output_type":"display_data","data":{"text/plain":["6*x*y*z"],"text/latex":"$\\displaystyle 6 x y z$"},"metadata":{}},{"output_type":"stream","name":"stdout","text":["divergence of F at (1,2,3) is\n","curl of F=\n"]},{"output_type":"display_data","data":{"text/plain":["x**2*y*z*v.x + x*y**2*z*v.y + x*y*z**2*v.z"],"text/latex":"$\\displaystyle x^{2} y z\\mathbf{\\hat{v}_x} + x y^{2} z\\mathbf{\\hat{v}_y} + x y z^{2}\\mathbf{\\hat{v}_z}$"},"metadata":{}},{"output_type":"stream","name":"stdout","text":["divergence of F at(1,2,3) is\n"]},{"output_type":"display_data","data":{"text/plain":["(-v_x*v_y**2 + v_x*v_z**2)*v.x + (v_x**2*v_y - v_y*v_z**2)*v.y + (-v_x**2*v_z + v_y**2*v_z)*v.z"],"text/latex":"$\\displaystyle (- v_{x} v_{y}^{2} + v_{x} v_{z}^{2})\\mathbf{\\hat{v}_x} + (v_{x}^{2} v_{y} - v_{y} v_{z}^{2})\\mathbf{\\hat{v}_y} + (- v_{x}^{2} v_{z} + v_{y}^{2} v_{z})\\mathbf{\\hat{v}_z}$"},"metadata":{}}]}]}